theories/lang/lang.v
@@ -1,367 +1,9 @@
 From iris.program_logic Require Export language ectx_language ectxi_language.
 From stdpp Require Export strings.
 From stdpp Require Import gmap list.
-From refinedc.lang Require Export base byte layout int_type.
+From refinedc.lang Require Export base byte layout int_type loc val heap.
 Set Default Proof Using "Type".
-
 Open Scope Z_scope.
-
-(** * Locations *)
-
-Declare Scope loc_scope.
-Delimit Scope loc_scope with L.
-Open Scope loc_scope.
-
-(** Physical address. *)
-Definition addr := Z.
-
-(** Allocation identifier (unique to an allocation). *)
-Definition alloc_id := Z.
-Definition dummy_alloc_id : alloc_id := 0.
-
-(** Memory location. *)
-Definition loc : Set := option alloc_id * addr.
-Bind Scope loc_scope with loc.
-
-Definition shift_loc (l : loc) (z : Z) : loc := (l.1, l.2 + z).
-Notation "l +ₗ z" := (shift_loc l%L z%Z)
-  (at level 50, left associativity) : loc_scope.
-Typeclasses Opaque shift_loc.
-
-Definition offset_loc (l : loc) (ly : layout) (z : Z) : loc := (l +ₗ ly.(ly_size) * z).
-Notation "l 'offset{' ly '}ₗ' z" := (offset_loc l%L ly z%Z)
-  (at level 50, format "l  'offset{' ly '}ₗ'  z", left associativity) : loc_scope.
-Typeclasses Opaque offset_loc.
-
-Definition aligned_to (l : loc) (n : nat) : Prop := (n | l.2).
-Notation "l `aligned_to` n" := (aligned_to l n) (at level 50) : stdpp_scope.
-Arguments aligned_to : simpl never.
-Typeclasses Opaque aligned_to.
-
-Definition has_layout_loc (l : loc) (ly : layout) : Prop := l `aligned_to` ly_align ly.
-Notation "l `has_layout_loc` n" := (has_layout_loc l n) (at level 50) : stdpp_scope.
-Arguments has_layout_loc : simpl never.
-Typeclasses Opaque has_layout_loc.
-
-Section loc_lemmas.
-  (*+ Lemmas about [shift_loc] and [offset_loc] *)
-  Lemma shift_loc_assoc l n1 n2 : l +ₗ n1 +ₗ n2 = l +ₗ (n1 + n2).
-  Proof. rewrite /shift_loc /=. f_equal. lia. Qed.
-
-  Lemma shift_loc_0 l : l +ₗ 0 = l.
-  Proof. destruct l as [??]. by rewrite /shift_loc Z.add_0_r. Qed.
-
-  Lemma shift_loc_assoc_nat l (n1 n2 : nat) : l +ₗ n1 +ₗ n2 = l +ₗ (n1 + n2)%nat.
-  Proof. rewrite /shift_loc /=. f_equal. lia. Qed.
-
-  Lemma shift_loc_0_nat l : l +ₗ 0%nat = l.
-  Proof. have: Z.of_nat 0%nat = 0 by lia. move => ->. apply shift_loc_0. Qed.
-
-  Lemma shift_loc_S l n: l +ₗ S n = (l +ₗ 1%nat +ₗ n).
-  Proof. by rewrite shift_loc_assoc_nat. Qed.
-
-  Lemma shift_loc_inj1 l1 l2 n : l1 +ₗ n = l2 +ₗ n → l1 = l2.
-  Proof. destruct l1, l2. case => -> ?. f_equal. lia. Qed.
-
-  Global Instance shift_loc_inj2 l : Inj (=) (=) (shift_loc l).
-  Proof. destruct l as [b o]; intros n n' [=?]; lia. Qed.
-
-  Lemma shift_loc_block l n : (l +ₗ n).1 = l.1.
-  Proof. done. Qed.
-
-  Lemma offset_loc_0 l ly : l offset{ly}ₗ 0 = l.
-  Proof. by rewrite /offset_loc Z.mul_0_r shift_loc_0. Qed.
-
-  Lemma offset_loc_S l ly n : l offset{ly}ₗ S n = (l offset{ly}ₗ 1) offset{ly}ₗ n.
-  Proof. destruct l. rewrite /offset_loc /shift_loc /=. f_equal. lia. Qed.
-
-  Lemma offset_loc_1 l ly : l offset{ly}ₗ 1%nat = (l +ₗ ly.(ly_size)).
-  Proof. destruct l. rewrite /offset_loc /shift_loc /=. f_equal. lia. Qed.
-
-  Lemma offset_loc_sz1 ly l n : ly.(ly_size) = 1%nat → l offset{ly}ₗ n = l +ₗ n.
-  Proof. rewrite /offset_loc => ->. f_equal. lia. Qed.
-
-  (*+ Lemmas about [aligned_to] and [has_layout_loc] *)
-  Lemma ly_with_align_aligned_to l m n:
-    l `aligned_to` n →
-    is_power_of_two n →
-    l `has_layout_loc` ly_with_align m n.
-  Proof. move => ??. by rewrite /has_layout_loc ly_align_ly_with_align keep_factor2_is_power_of_two. Qed.
-
-  Lemma has_layout_loc_trans l ly1 ly2 :
-    l `has_layout_loc` ly2 → (ly1.(ly_align_log) ≤ ly2.(ly_align_log))%nat → l `has_layout_loc` ly1.
-  Proof. rewrite /has_layout_loc/aligned_to => Hl ?. etrans;[|by apply Hl]. by apply Zdivide_nat_pow. Qed.
-
-  Lemma has_layout_loc_trans' l ly1 ly2 :
-    l `has_layout_loc` ly2 → (ly_align ly1 ≤ ly_align ly2)%nat → l `has_layout_loc` ly1.
-  Proof. rewrite -ly_align_log_ly_align_le_iff. by apply: has_layout_loc_trans. Qed.
-
-  Lemma has_layout_loc_1 l ly:
-    ly_align ly = 1%nat →
-    l `has_layout_loc` ly.
-  Proof. rewrite /has_layout_loc =>  ->. by apply Z.divide_1_l. Qed.
-
-  Lemma has_layout_ly_offset l (n : nat) ly:
-    l `has_layout_loc` ly →
-    (l +ₗ n) `has_layout_loc` ly_offset ly n.
-  Proof.
-    move => Hl. apply Z.divide_add_r.
-    - apply: has_layout_loc_trans => //. rewrite {1}/ly_align_log/=. destruct n; lia.
-    - rewrite/ly_offset. destruct n;[by subst;apply Z.divide_0_r|]. etrans;[apply Zdivide_nat_pow, Min.le_min_r|].   by apply factor2_divide.
-  Qed.
-
-  Lemma has_layout_loc_ly_mult_offset l ly n:
-    layout_wf ly →
-    l `has_layout_loc` ly_mult ly (S n) →
-    (l +ₗ ly_size ly) `has_layout_loc` ly_mult ly n.
-  Proof. move => ??. rewrite /ly_mult. by apply Z.divide_add_r. Qed.
-
-
-  Lemma aligned_to_offset l n off :
-    l `aligned_to` n → (n | off) → (l +ₗ off) `aligned_to` n.
-  Proof. apply Z.divide_add_r. Qed.
-
-  Lemma aligned_to_add l (n : nat) x:
-    (l +ₗ x * n) `aligned_to` n ↔ l `aligned_to` n.
-  Proof.
-    unfold aligned_to. destruct l => /=. rewrite Z.add_comm.
-    split.
-    - apply: Z.divide_add_cancel_r. by apply Z.divide_mul_r.
-    - apply Z.divide_add_r. by apply Z.divide_mul_r.
-  Qed.
-
-  Lemma aligned_to_mult_eq l n1 n2 off:
-    l `aligned_to` n2 → (l +ₗ off) `aligned_to` (n1 * n2) → (n2 | off).
-  Proof.
-    unfold aligned_to. destruct l => /= ??. apply: Z.divide_add_cancel_r => //.
-    apply: (Zdivide_mult_l _ n1). by rewrite Z.mul_comm -Nat2Z.inj_mul.
-  Qed.
-End loc_lemmas.
-
-(** * Bytes and values stored in memory *)
-
-(** Representation of a byte stored in memory. *)
-Inductive mbyte : Set :=
-| MByte (b : byte)
-| MPtrFrag (l : loc) (n : nat)
-| MPoison.
-
-(** Representation of a value (list of bytes). *)
-Definition val : Set := list mbyte.
-Bind Scope val_scope with val.
-
-Definition has_layout_val (v : val) (ly : layout) : Prop := length v = ly.(ly_size).
-Notation "v `has_layout_val` n" := (has_layout_val v n) (at level 50) : stdpp_scope.
-Arguments has_layout_val : simpl never.
-Typeclasses Opaque has_layout_val.
-
-(** * Representation of the heap *)
-
-Inductive lock_state := WSt | RSt (n : nat).
-
-Record heap_cell := HeapCell {
-  hc_alloc_id   : alloc_id;   (** Allocation owning the cell. *)
-  hc_lock_state : lock_state; (** Datarace detection stuff. *)
-  hc_value      : mbyte;      (** Byte value. *)
-}.
-
-Definition heap := gmap addr heap_cell.
-
-(** Predicate stating that the heap [h] contains value [v] at address [a],
-and that every cell involved has an allocation identifier and a lock state
-that satisfy [Paid] and [Plk] respectively. *)
-Fixpoint heap_lookup (a : addr) (v : val) (Paid : alloc_id → Prop)
-                       (Plk : lock_state → Prop) (h : heap) : Prop :=
-  match v with
-  | []     => True
-  | b :: v => (∃ aid lk, h !! a = Some (HeapCell aid lk b) ∧ Paid aid ∧ Plk lk) ∧
-              heap_lookup (Z.succ a) v Paid Plk h
-  end.
-
-(** Function writing value [v] at address [a] in heap [h]. For all involved
-cells in the resulting heap, an allocation id and lock state is built using
-functions [faid] and [flk] respectively. These functions receive as input
-the previous value of the field (if the cell previously existed in [h]). *)
-Fixpoint heap_update (a : addr) (v : val) (faid : option alloc_id → alloc_id)
-                     (flk : option lock_state → lock_state) (h : heap) : heap :=
-  match v with
-  | []     => h
-  | b :: v => let update m :=
-                Some {|
-                  hc_alloc_id   := faid (hc_alloc_id <$> m);
-                  hc_lock_state := flk (hc_lock_state <$> m);
-                  hc_value      := b;
-                |}
-              in
-              partial_alter update a (heap_update (Z.succ a) v faid flk h)
-  end.
-
-Definition heap_lookup_loc (l : loc) (v : val) (Plk : lock_state → Prop)
-                             (h : heap) : Prop :=
-  heap_lookup l.2 v (λ aid, l.1 = Some aid) Plk h.
-
-Definition heap_alloc (a : addr) (v : val) (aid : alloc_id) (h : heap) : heap :=
-  heap_update a v (λ _, aid) (λ _, RSt 0%nat) h.
-
-(** Predicate stating that the allocation [aid] is still present in heap [h]. *)
-Definition heap_block_alive (h : heap) (aid : alloc_id) : Prop :=
-  ∃ a, hc_alloc_id <$> h !! a = Some aid.
-
-Definition heap_at (l : loc) (ly : layout) (v : val) (Plk : lock_state → Prop)
-                   (h : heap) : Prop :=
-  is_Some l.1 ∧ l `has_layout_loc` ly ∧ v `has_layout_val` ly ∧
-  heap_lookup_loc l v Plk h.
-
-Definition heap_upd l v flk h :=
-  heap_update l.2 v (λ _, default dummy_alloc_id l.1) flk h.
-
-(** Predicate stating that the [n] first bytes from address [a] in [h] have
-not been allocated. *)
-Definition heap_range_free (h : heap) (a : addr) (n : nat) : Prop :=
-  ∀ a', a ≤ a' < a + n → h !! a' = None.
-
-(** Free [n] cells starting at [a] in [h]. *)
-Fixpoint heap_free (a : addr) (n : nat) (h : heap) : heap :=
-  match n with
-  | O   => h
-  | S n => delete a (heap_free (Z.succ a) n h)
-  end.
-
-Fixpoint heap_free_list (ls : list (loc * layout)) (h : heap) : heap :=
-  match ls with
-  | []           => h
-  | (l,ly) :: ls => heap_free l.2 ly.(ly_size) (heap_free_list ls h)
-  end.
-
-Section heap_lemmas.
-  Lemma heap_lookup_inj_val a h v1 v2 Paid1 Paid2 Plk1 Plk2:
-    length v1 = length v2 →
-    heap_lookup a v1 Paid1 Plk1 h → heap_lookup a v2 Paid2 Plk2 h → v1 = v2.
-  Proof.
-    elim: v1 v2 a; first by move => [|??] //.
-    move => ?? IH [|??] //= ? [?] [[?[?[??]]]?] [[?[?[??]]]?]; simplify_eq.
-    f_equal. by apply: IH.
-  Qed.
-
-  Lemma heap_update_ext h a v faid1 faid2 flk1 flk2:
-    (∀ x, faid1 x = faid2 x) → (∀ x, flk1 x = flk2 x) →
-    heap_update a v faid1 flk1 h = heap_update a v faid2 flk2 h.
-  Proof.
-    move => Hext1 Hext2. elim: v a => //= ?? IH ?. rewrite IH.
-    apply: partial_alter_ext => ??. by rewrite Hext1 Hext2.
-  Qed.
-
-  Lemma heap_update_lookup_lt a1 a2 v faid flk h:
-    a1 < a2 →
-    heap_update a2 v faid flk h !! a1 = h !! a1.
-  Proof.
-    elim: v a1 a2 => // ?? IH ???.
-    rewrite lookup_partial_alter_ne; last lia. apply IH. lia.
-  Qed.
-
-  Lemma heap_free_delete h a1 a2 n :
-    delete a1 (heap_free a2 n h) = heap_free a2 n (delete a1 h).
-  Proof. elim: n a2 => //= ? IH ?. by rewrite delete_commute IH. Qed.
-
-  Lemma heap_free_list_app ls1 ls2 h :
-    heap_free_list (ls1 ++ ls2) h = heap_free_list ls1 (heap_free_list ls2 h).
-  Proof. by elim: ls1 => //= [[??]] ? ->. Qed.
-
-  Lemma heap_upd_ext h l v f1 f2:
-    (∀ x, f1 x = f2 x) → heap_upd l v f1 h = heap_upd l v f2 h.
-  Proof. by apply heap_update_ext. Qed.
-
-  Lemma heap_at_inj_val l ly h v1 v2 Plk1 Plk2:
-    heap_at l ly v1 Plk1 h → heap_at l ly v2 Plk2 h → v1 = v2.
-  Proof.
-    move => [_[?[??]]] [_[?[??]]].
-    apply: heap_lookup_inj_val => //. congruence.
-  Qed.
-
-  Lemma heap_lookup_loc_inj_val  l h v v' flk1 flk2 ly:
-    v `has_layout_val` ly →
-    heap_lookup_loc l v flk1 h → heap_at l ly v' flk2 h → v = v'.
-  Proof.
-    move => ??[_[?[??]]]. apply: heap_lookup_inj_val => //. congruence.
-  Qed.
-
-  Lemma heap_upd_heap_at_id l v flk flk' h:
-    heap_lookup_loc l v flk' h →
-    (∀ st, flk (Some st) = st) →
-    heap_upd l v flk h = h.
-  Proof.
-    rewrite /heap_upd.
-    elim: v l => // ?? IH ? [[?[?[H[H1 ?]]]]?] Hlookup /=.
-    assert (∀ l, Z.succ l.2 = (l +ₗ 1).2) as -> by done.
-    rewrite IH => //. apply: partial_alter_self_alt'.
-    by rewrite H Hlookup H1 /=.
-  Qed.
-End heap_lemmas.
-
-(** * Allocations and heap state *)
-
-Record allocation :=
-  Allocation {
-    alloc_start : Z; (* First valid address. *)
-    alloc_end : Z;   (* One-past-the-end address. *)
-  }.
-
-Definition allocs := gmap alloc_id allocation.
-
-Record heap_state := {
-  hs_heap   : heap;
-  hs_allocs : allocs;
-}.
-
-(** Smallest allocatble address (we reserve 0 for NULL). *)
-Definition min_alloc_start : Z := 1.
-
-(** Largest allocatable address (we never allocate the last byte to always
-have valid one-past pointers. *)
-Definition max_alloc_end : Z := 2 ^ (bytes_per_addr * bits_per_byte) - 2.
-
-Definition to_allocation (off : Z) (len : nat) : allocation :=
-  Allocation off (off + len).
-
-Definition allocation_in_range (a : allocation) : Prop :=
-  min_alloc_start ≤ a.(alloc_start) ∧ a.(alloc_end) ≤ max_alloc_end.
-
-(** The address range between [l] and [l +ₗ n] (included) is in range of the
-    allocation that contains [l]. Note that we consider the 1-past-the-end
-    pointer to be in range of an allocation. *)
-Definition heap_state_loc_in_bounds (l : loc) (n : nat) (st : heap_state) : Prop :=
-  ∃ alloc_id alloc,
-    l.1 = Some alloc_id ∧
-    st.(hs_allocs) !! alloc_id = Some alloc ∧
-    alloc.(alloc_start) ≤ l.2 ∧
-    l.2 + n ≤ alloc.(alloc_end).
-
-(** Checks that the location [l] is inbounds of its allocation
-(one-past-the-end is allowed) and this allocation is still alive *)
-Definition valid_ptr (l : loc) (st : heap_state) : Prop :=
-  ∃ aid, l.1 = Some aid ∧ heap_block_alive st.(hs_heap) aid ∧ heap_state_loc_in_bounds l 0 st.
-
-Inductive alloc_new_block : heap_state → loc → val → heap_state → Prop :=
-| AllocNewBlock σ l aid v:
-    l.1 = Some aid →
-    σ.(hs_allocs) !! aid = None →
-    (* TODO: is the precondition really useful? It should follow from
-    the previous. *)
-    ¬ heap_block_alive σ.(hs_heap) aid →
-    allocation_in_range (to_allocation l.2 (length v)) →
-    heap_range_free σ.(hs_heap) l.2 (length v) →
-    alloc_new_block σ l v {|
-      hs_heap   := heap_alloc l.2 v aid σ.(hs_heap);
-      hs_allocs := <[aid := to_allocation l.2 (length v)]> σ.(hs_allocs);
-    |}.
-
-Inductive alloc_new_blocks : heap_state → list loc → list val → heap_state → Prop :=
-| AllocNewBlock_nil σ :
-    alloc_new_blocks σ [] [] σ
-| AllocNewBlock_cons σ σ' σ'' l v ls vs :
-    alloc_new_block σ l v σ' →
-    alloc_new_blocks σ' ls vs σ'' →
-    alloc_new_blocks σ (l :: ls) (v :: vs) σ''.
 
 (** * Definition of the language *)
 
@@ -539,155 +181,7 @@ Qed.
 Global Instance to_rtstmt_inj : Inj2 (=) (=) (=) to_rtstmt.
 Proof. move => ? s1 ? s2 [-> ]. elim: s1 s2 => [ ^ e1 ] [ ^ e2 ] // ?; simplify_eq => //. Qed.
 
-Implicit Type (l : loc) (re : rtexpr) (v : val) (sz : nat) (h : heap) (σ : state) (ly : layout) (rs : rtstmt) (s : stmt) (sgn : signed) (rf : runtime_function).
-
-(*** Relating val to logical values *)
-(*+ [val_to_int] and [val_of_int] *)
-(* we use little endian *)
-Fixpoint val_to_int_go v : option Z :=
-match v with
-| [] => Some 0
-| (MByte b)::v' => z ← val_to_int_go v'; Some (byte_modulus * z + b.(byte_val))
-| _ => None
-end.
-Definition val_to_int (v : val) (it : int_type) : option Z :=
-  if decide (length v = bytes_per_int it) then
-    z ← val_to_int_go v; if it.(it_signed) && bool_decide (int_half_modulus it ≤ z) then Some (z - int_modulus it) else Some z
-  else None.
-
-Program Fixpoint val_of_int_go (n : Z) sz : val :=
-  match sz return _ with
-  | O => []
-  | S sz' => (MByte ({| byte_val := (n `mod` byte_modulus) |}))::(val_of_int_go (n / byte_modulus) sz')
-  end.
-Next Obligation. move => n. have [] := Z_mod_lt n byte_modulus => //*. lia. Qed.
-
-Definition val_of_int (z : Z) (it : int_type) : option val :=
-  if bool_decide (z ∈ it) then
-    let p := if bool_decide (z < 0) then z + int_modulus it else z in
-    Some (val_of_int_go p (bytes_per_int it))
-  else
-    None.
-
-Lemma val_of_int_go_length z sz :
-  length (val_of_int_go z sz) = sz.
-Proof. elim: sz z => //= ? IH ?. by f_equal. Qed.
-
-Lemma val_to_of_int_go z sz :
-  0 ≤ z < 2 ^ (sz * bits_per_byte) →
-  val_to_int_go (val_of_int_go z sz) = Some z.
-Proof.
-  rewrite /bits_per_byte.
-  elim: sz z => /=. 1: rewrite /Z.of_nat; move => ??; f_equal; lia.
-  move => sz IH z [? Hlt]. rewrite IH /byte_modulus /= -?Z_div_mod_eq //.
-  split. apply Z_div_pos => //. apply Zdiv_lt_upper_bound => //.
-  rewrite Nat2Z.inj_succ -Zmult_succ_l_reverse Z.pow_add_r // in Hlt.
-  lia.
-Qed.
-
-Lemma val_of_int_length z it v:
-  val_of_int z it = Some v → length v = bytes_per_int it.
-Proof. rewrite /val_of_int => Hv. case_bool_decide => //. simplify_eq. by rewrite val_of_int_go_length. Qed.
-
-Lemma val_to_int_length v it z:
-  val_to_int v it = Some z → length v = bytes_per_int it.
-Proof. rewrite /val_to_int. by case_decide. Qed.
-
-Lemma val_of_int_is_some it z:
-  z ∈ it → is_Some (val_of_int z it).
-Proof. rewrite /val_of_int. case_bool_decide; by eauto. Qed.
-
-Lemma val_of_int_in_range it z v:
-  val_of_int z it = Some v → z ∈ it.
-Proof. rewrite /val_of_int. case_bool_decide; by eauto. Qed.
-
-Lemma val_to_of_int z it v:
-  val_of_int z it = Some v → val_to_int v it = Some z.
-Proof.
-  rewrite /val_of_int /val_to_int => Ht.
-  destruct (bool_decide (z ∈ it)) eqn: Hr => //. simplify_eq.
-  move: Hr => /bool_decide_eq_true[Hm HM].
-  have Hlen := bytes_per_int_gt_0 it.
-  rewrite /max_int in HM. rewrite /min_int in Hm.
-  rewrite val_of_int_go_length val_to_of_int_go /=.
-  - case_decide as H => //. clear H.
-    destruct (it_signed it) eqn:Hs => /=.
-    + case_decide => /=; last (rewrite bool_decide_false //; lia).
-      rewrite bool_decide_true; [f_equal; lia|].
-      rewrite int_modulus_twice_half_modulus. move: Hm HM.
-      generalize (int_half_modulus it). move => n Hm HM. lia.
-    + rewrite bool_decide_false //. lia.
-  - case_bool_decide as Hneg; case_match; split; try lia.
-    + rewrite int_modulus_twice_half_modulus. lia.
-    + rewrite /int_modulus /bits_per_int. lia.
-    + rewrite /int_half_modulus in HM.
-      transitivity (2 ^ (bits_per_int it -1)); first lia.
-      rewrite /bits_per_int /bytes_per_int /bits_per_byte /=.
-      apply Z.pow_lt_mono_r; try lia.
-    + rewrite /int_modulus /bits_per_int in HM. lia.
-Qed.
-
-(*+ [val_to_loc] and [val_of_loc] *)
-Fixpoint val_to_loc_go (v : val) (pos : nat) (l : loc) : option loc :=
-  match v with
-  | (MPtrFrag l' pos')::v' =>
-    if bool_decide (pos = pos' ∧ l = l') then
-      if bool_decide (pos = bytes_per_addr - 1)%nat then (if v' is [] then Some l else None) else val_to_loc_go v' (S pos) l
-    else None
-  | _ => None
-  end.
-Definition val_to_loc (v : val) : option loc :=
-  match v with
-  | (MPtrFrag l 0)::v' => val_to_loc_go v' 1%nat l
-  | _ => None
-  end.
-Definition val_of_loc (l : loc) : val := MPtrFrag l <$> seq 0 bytes_per_addr.
-
-Lemma val_to_of_loc l :
-  val_to_loc (val_of_loc l) = Some l.
-Proof. simpl. by case_decide. Qed.
-
-Lemma val_of_to_loc v l :
-  val_to_loc v = Some l → v = val_of_loc l.
-Proof.
-  destruct v => //=; case_match => //; case_match => //.
-  repeat (match goal with
-  | |- context [ val_to_loc_go ?v _ _ ] => destruct v
-          end => //=;
-                  case_match => //; repeat (case_decide; subst => //=)).
-  by case_match => // [[->]].
-Qed.
-
-(*+ [val_of_bool] and [i2v] *)
-Definition i2v (n : Z) (it : int_type) : val := default [MPoison] (val_of_int n it).
-
-Definition val_of_bool (b : bool) : val := i2v (Z_of_bool b) bool_it.
-
-Lemma val_of_int_bool b it:
-  val_of_int (Z_of_bool b) it = Some (i2v (Z_of_bool b) it).
-Proof.
-  have [|? Hv] := val_of_int_is_some it (Z_of_bool b); last by rewrite /i2v Hv.
-  rewrite /elem_of /int_elem_of_it.
-  have ? := min_int_le_0 it. have ? := max_int_ge_127 it.
-  split; destruct b => /=; lia.
-Qed.
-
-Lemma val_to_int_bool b :
-  val_to_int (val_of_bool b) bool_it = Some (Z_of_bool b).
-Proof. by destruct b. Qed.
-
-Lemma i2v_bool_length b it:
-  length (i2v (Z_of_bool b) it) = bytes_per_int it.
-Proof. by have /val_of_int_length -> := val_of_int_bool b it. Qed.
-Lemma i2v_bool_Some b it:
-  val_to_int (i2v (Z_of_bool b) it) it = Some (Z_of_bool b).
-Proof. apply val_to_of_int. apply val_of_int_bool. Qed.
-
-Arguments val_to_int : simpl never.
-Arguments val_of_int : simpl never.
-Arguments val_to_loc : simpl never.
-Arguments val_of_loc : simpl never.
-Typeclasses Opaque val_to_loc val_of_loc val_to_int val_of_int val_of_bool.
+Implicit Type (l : loc) (re : rtexpr) (v : val) (h : heap) (σ : state) (ly : layout) (rs : rtstmt) (s : stmt) (sgn : signed) (rf : runtime_function).
 
 (*** Substitution *)
 Fixpoint subst (x : var_name) (v : val) (e : expr)  : expr :=
@@ -855,6 +349,9 @@ Inductive eval_un_op : un_op → op_type → state → val → val → Prop :=
 
 (*** Evaluation of Expressions *)
 
+Definition state_alloc_new_blocks (σ1 : state) (ls : list loc) (vs : list val) (σ2 : state) : Prop :=
+  alloc_new_blocks σ1.(st_heap) ls vs σ2.(st_heap) ∧ σ1.(st_fntbl) = σ2.(st_fntbl).
+
 Inductive expr_step : expr → state → list Empty_set → runtime_expr → state → list runtime_expr → Prop :=
 | SkipES v σ:
     expr_step (SkipE (Val v)) σ [] (Val v) σ []
@@ -918,11 +415,9 @@ comparing pointers? (see lambda rust) *)
     Forall2 has_layout_loc lsa fn.(f_args).*2 →
     Forall2 has_layout_loc lsv fn.(f_local_vars).*2 →
     (* initialize the local vars to poison *)
-    alloc_new_blocks σ.(st_heap) lsv ((λ p, replicate p.2.(ly_size) MPoison) <$> fn.(f_local_vars)) σ'.(st_heap) →
-    σ.(st_fntbl) = σ'.(st_fntbl) →
+    state_alloc_new_blocks σ lsv ((λ p, replicate p.2.(ly_size) MPoison) <$> fn.(f_local_vars)) σ' →
     (* initialize the arguments with the supplied values *)
-    alloc_new_blocks σ'.(st_heap) lsa vs σ''.(st_heap) →
-    σ'.(st_fntbl) = σ''.(st_fntbl) →
+    state_alloc_new_blocks σ' lsa vs σ'' →
     (* add used blocks allocations  *)
     rf = {| rf_fn := fn'; rf_locs := zip lsa fn.(f_args).*2 ++ zip lsv fn.(f_local_vars).*2; |} →
     expr_step (Call (Val vf) (Val <$> vs)) σ [] (to_rtstmt rf (Goto fn'.(f_init))) σ'' []
@@ -961,10 +456,9 @@ Inductive stmt_step : stmt → runtime_function → state → list Empty_set →
 | GotoS rf σ b s :
     rf.(rf_fn).(f_code) !! b = Some s →
     stmt_step (Goto b) rf σ [] (to_rtstmt rf s) σ []
-| ReturnS rf σ v:
-    stmt_step (Return (Val v)) rf σ [] (Val v)
-     (* deallocate the stack *)
-     (heap_fmap (heap_free_list rf.(rf_locs)) σ) []
+| ReturnS rf σ hs v:
+    free_blocks σ.(st_heap) rf.(rf_locs) hs → (* Deallocate the stack. *)
+    stmt_step (Return (Val v)) rf σ [] (Val v) {| st_fntbl := σ.(st_fntbl); st_heap := hs |} []
 | SkipSS rf σ s :
     stmt_step (SkipS s) rf σ [] (to_rtstmt rf s) σ []
 | ExprSS rf σ s v:
@@ -983,6 +477,43 @@ Inductive runtime_step : runtime_expr → state → list Empty_set → runtime_e
 | AllocFailedStep σ :
     (* Alloc failure is nb, not ub so we go into an infinite loop*)
     runtime_step AllocFailed σ [] AllocFailed σ [].
+
+Lemma expr_step_preserves_invariant e1 e2 σ1 σ2 κs efs:
+  expr_step e1 σ1 κs e2 σ2 efs →
+  heap_state_invariant σ1.(st_heap) →
+  heap_state_invariant σ2.(st_heap).
+Proof.
+  move => [] // *.
+  all: repeat select (heap_at _ _ _ _ _) ltac:(fun H => destruct H as [?[?[??]]]).
+  all: try (rewrite /heap_fmap/=; eapply heap_update_heap_state_invariant => //).
+  all: try (unfold has_layout_val in *; by etransitivity).
+  repeat match goal with H : state_alloc_new_blocks _ _ _ _ |- _ => destruct H as [??] end.
+  repeat eapply alloc_new_blocks_invariant => //.
+Qed.
+
+Lemma stmt_step_preserves_invariant s rf e σ1 σ2 κs efs:
+  stmt_step s rf σ1 κs e σ2 efs →
+  heap_state_invariant σ1.(st_heap) →
+  heap_state_invariant σ2.(st_heap).
+Proof.
+  move => [] //; clear.
+  - move => o *.
+    revert select (heap_at _ _ _ _ _) => -[?[?[??]]].
+    rewrite /heap_fmap/=. eapply heap_update_heap_state_invariant => //.
+    match goal with H : _ `has_layout_val` _ |- _ => try rewrite H // end.
+    by destruct o.
+  - move => ??? _ Hfree Hinv. by eapply free_blocks_invariant.
+Qed.
+
+Lemma runtime_step_preserves_invariant e1 e2 σ1 σ2 κs efs:
+  runtime_step e1 σ1 κs e2 σ2 efs →
+  heap_state_invariant σ1.(st_heap) →
+  heap_state_invariant σ2.(st_heap).
+Proof.
+  move => [] // *.
+  - by eapply expr_step_preserves_invariant.
+  - by eapply stmt_step_preserves_invariant.
+Qed.
 
 (*** evaluation contexts *)
 (** for expressions*)
