theories/lang/val.v
@@ -1,0 +1,189 @@
+From refinedc.lang Require Export base byte layout int_type loc.
+Set Default Proof Using "Type".
+Open Scope Z_scope.
+
+(** * Bytes and values stored in memory *)
+
+(** Representation of a byte stored in memory. *)
+Inductive mbyte : Set :=
+| MByte (b : byte)
+| MPtrFrag (l : loc) (n : nat)
+| MPoison.
+
+(** Representation of a value (list of bytes). *)
+Definition val : Set := list mbyte.
+Bind Scope val_scope with val.
+
+(** Predicate stating that value [v] has the right size according to layout [ly]. *)
+Definition has_layout_val (v : val) (ly : layout) : Prop := length v = ly.(ly_size).
+Notation "v `has_layout_val` n" := (has_layout_val v n) (at level 50) : stdpp_scope.
+Arguments has_layout_val : simpl never.
+Typeclasses Opaque has_layout_val.
+
+(** ** Conversion to and from mathematical integers. *)
+
+(* TODO: we currently assume little-endian, make this more generic. *)
+
+Fixpoint val_to_int_go v : option Z :=
+  match v with
+  | []           => Some 0
+  | MByte b :: v => z ← val_to_int_go v; Some (byte_modulus * z + b.(byte_val))
+  | _            => None
+  end.
+
+Definition val_to_int (v : val) (it : int_type) : option Z :=
+  if decide (length v = bytes_per_int it) then
+    z ← val_to_int_go v;
+    if it.(it_signed) && bool_decide (int_half_modulus it ≤ z) then
+      Some (z - int_modulus it)
+    else
+      Some z
+  else None.
+
+Program Fixpoint val_of_int_go (n : Z) (sz : nat) : val :=
+  match sz return _ with
+  | O    => []
+  | S sz => MByte {| byte_val := (n `mod` byte_modulus) |}
+            :: val_of_int_go (n / byte_modulus) sz
+  end.
+Next Obligation. move => n. have [] := Z_mod_lt n byte_modulus => //*. lia. Qed.
+
+Definition val_of_int (z : Z) (it : int_type) : option val :=
+  if bool_decide (z ∈ it) then
+    let p := if bool_decide (z < 0) then z + int_modulus it else z in
+    Some (val_of_int_go p (bytes_per_int it))
+  else
+    None.
+
+Definition i2v (n : Z) (it : int_type) : val :=
+  default [MPoison] (val_of_int n it).
+
+Definition val_of_bool (b : bool) : val :=
+  i2v (Z_of_bool b) bool_it.
+
+Lemma val_of_int_go_length z sz :
+  length (val_of_int_go z sz) = sz.
+Proof. elim: sz z => //= ? IH ?. by f_equal. Qed.
+
+Lemma val_to_of_int_go z (sz : nat) :
+  0 ≤ z < 2 ^ (sz * bits_per_byte) →
+  val_to_int_go (val_of_int_go z sz) = Some z.
+Proof.
+  rewrite /bits_per_byte.
+  elim: sz z => /=. 1: rewrite /Z.of_nat; move => ??; f_equal; lia.
+  move => sz IH z [? Hlt]. rewrite IH /byte_modulus /= -?Z_div_mod_eq //.
+  split. apply Z_div_pos => //. apply Zdiv_lt_upper_bound => //.
+  rewrite Nat2Z.inj_succ -Zmult_succ_l_reverse Z.pow_add_r // in Hlt.
+  lia.
+Qed.
+
+Lemma val_of_int_length z it v:
+  val_of_int z it = Some v → length v = bytes_per_int it.
+Proof.
+  rewrite /val_of_int => Hv. case_bool_decide => //. simplify_eq.
+  by rewrite val_of_int_go_length.
+Qed.
+
+Lemma val_to_int_length v it z:
+  val_to_int v it = Some z → length v = bytes_per_int it.
+Proof. rewrite /val_to_int. by case_decide. Qed.
+
+Lemma val_of_int_is_some it z:
+  z ∈ it → is_Some (val_of_int z it).
+Proof. rewrite /val_of_int. case_bool_decide; by eauto. Qed.
+
+Lemma val_of_int_in_range it z v:
+  val_of_int z it = Some v → z ∈ it.
+Proof. rewrite /val_of_int. case_bool_decide; by eauto. Qed.
+
+Lemma val_to_of_int z it v:
+  val_of_int z it = Some v → val_to_int v it = Some z.
+Proof.
+  rewrite /val_of_int /val_to_int => Ht.
+  destruct (bool_decide (z ∈ it)) eqn: Hr => //. simplify_eq.
+  move: Hr => /bool_decide_eq_true[Hm HM].
+  have Hlen := bytes_per_int_gt_0 it.
+  rewrite /max_int in HM. rewrite /min_int in Hm.
+  rewrite val_of_int_go_length val_to_of_int_go /=.
+  - case_decide as H => //. clear H.
+    destruct (it_signed it) eqn:Hs => /=.
+    + case_decide => /=; last (rewrite bool_decide_false //; lia).
+      rewrite bool_decide_true; [f_equal; lia|].
+      rewrite int_modulus_twice_half_modulus. move: Hm HM.
+      generalize (int_half_modulus it). move => n Hm HM. lia.
+    + rewrite bool_decide_false //. lia.
+  - case_bool_decide as Hneg; case_match; split; try lia.
+    + rewrite int_modulus_twice_half_modulus. lia.
+    + rewrite /int_modulus /bits_per_int. lia.
+    + rewrite /int_half_modulus in HM.
+      transitivity (2 ^ (bits_per_int it -1)); first lia.
+      rewrite /bits_per_int /bytes_per_int /bits_per_byte /=.
+      apply Z.pow_lt_mono_r; try lia.
+    + rewrite /int_modulus /bits_per_int in HM. lia.
+Qed.
+
+Lemma val_of_int_bool b it:
+  val_of_int (Z_of_bool b) it = Some (i2v (Z_of_bool b) it).
+Proof.
+  have [|? Hv] := val_of_int_is_some it (Z_of_bool b); last by rewrite /i2v Hv.
+  rewrite /elem_of /int_elem_of_it.
+  have ? := min_int_le_0 it. have ? := max_int_ge_127 it.
+  split; destruct b => /=; lia.
+Qed.
+
+Lemma val_to_int_bool b :
+  val_to_int (val_of_bool b) bool_it = Some (Z_of_bool b).
+Proof. by destruct b. Qed.
+
+Lemma i2v_bool_length b it:
+  length (i2v (Z_of_bool b) it) = bytes_per_int it.
+Proof. by have /val_of_int_length -> := val_of_int_bool b it. Qed.
+
+Lemma i2v_bool_Some b it:
+  val_to_int (i2v (Z_of_bool b) it) it = Some (Z_of_bool b).
+Proof. apply val_to_of_int. apply val_of_int_bool. Qed.
+
+(** ** Conversion to and from locations. *)
+
+Fixpoint val_to_loc_go (v : val) (pos : nat) (l : loc) : option loc :=
+  match v with
+  | MPtrFrag l' pos' :: v =>
+      if bool_decide (pos = pos' ∧ l = l') then
+        if bool_decide (pos = bytes_per_addr - 1)%nat then
+          if v is [] then Some l else None
+        else
+          val_to_loc_go v (S pos) l
+      else
+        None
+  | _                     => None
+  end.
+
+Definition val_to_loc (v : val) : option loc :=
+  match v with
+  | MPtrFrag l 0 :: v => val_to_loc_go v 1 l
+  | _                 => None
+  end.
+
+Definition val_of_loc (l : loc) : val :=
+  MPtrFrag l <$> seq 0 bytes_per_addr.
+
+Lemma val_to_of_loc l :
+  val_to_loc (val_of_loc l) = Some l.
+Proof. simpl. by case_decide. Qed.
+
+Lemma val_of_to_loc v l :
+  val_to_loc v = Some l → v = val_of_loc l.
+Proof.
+  destruct v => //=; case_match => //; case_match => //.
+  repeat (match goal with
+  | |- context [ val_to_loc_go ?v _ _ ] => destruct v
+          end => //=;
+                  case_match => //; repeat (case_decide; subst => //=)).
+  by case_match => // [[->]].
+Qed.
+
+Arguments val_to_int : simpl never.
+Arguments val_of_int : simpl never.
+Arguments val_to_loc : simpl never.
+Arguments val_of_loc : simpl never.
+Typeclasses Opaque val_to_loc val_of_loc val_to_int val_of_int val_of_bool.
