theories/typing/programs.v
@@ -453,7 +453,7 @@ Section typing.
   Global Instance related_to_loc l β ty : RelatedTo (l ◁ₗ{β} ty) := {| rt_fic := FindLoc l |}.
   Global Instance related_to_val v ty `{!Movable ty} : RelatedTo (v ◁ᵥ ty) := {| rt_fic := FindValP v |}.
   Global Instance related_to_loc_in_bounds l n : RelatedTo (loc_in_bounds l n) := {| rt_fic := FindLocInBounds l |}.
-  Global Instance related_to_alloc_alive l : RelatedTo (alloc_alive l) := {| rt_fic := FindLoc l |}.
+  Global Instance related_to_alloc_alive l : RelatedTo (alloc_alive_loc l) := {| rt_fic := FindLoc l |}.
 
   Lemma subsume_loc_in_bounds ty β l (n m : nat) `{!LocInBounds ty β m} T :
     (l ◁ₗ{β} ty -∗ ⌜n ≤ m⌝ ∗ T) -∗
@@ -471,10 +471,10 @@ Section typing.
   Lemma subsume_alloc_alive ty β l P `{!AllocAlive ty β P} T :
     (* You don't get l ◁ₗ{β} ty back because alloc_alive is not persistent. *)
     P ∗ T -∗
-    subsume (l ◁ₗ{β} ty) (alloc_alive l) T.
+    subsume (l ◁ₗ{β} ty) (alloc_alive_loc l) T.
   Proof. iIntros "[HP $] Hl". by iApply (alloc_alive_alive with "HP"). Qed.
   Global Instance subsume_alloc_alive_inst ty β l P `{!AllocAlive ty β P} :
-    Subsume (l ◁ₗ{β} ty) (alloc_alive l) :=
+    Subsume (l ◁ₗ{β} ty) (alloc_alive_loc l) :=
     λ T, i2p (subsume_alloc_alive ty β l P T).
 
   Lemma subsume_loc_in_bounds_leq (l : loc) (n1 n2 : nat) T :
